New stuff

PractiseLean/Chap9.lean
@@ -42,4 +42,57 @@ inductive BigStep : Stmt × State → State → Prop where
     BigStep (Stmt.whileDo B S, s) s
 
 
+infix:110 " ⟹ " => BigStep
+
+inductive SmallStep : Stmt × State → Stmt × State → Prop where
+  | assign (x a s) :
+    SmallStep (Stmt.assign x a, s) (Stmt.skip, s[x ↦ a s])
+  | seq_step (S S' T s s') (hS : SmallStep (S, s) (S', s')) :
+    SmallStep (S; T, s) (S'; T, s')
+  | seq_skip (T s) :
+    SmallStep (Stmt.skip; T, s) (T, s)
+  | if_true (B S T s) (hcond : B s) :
+    SmallStep (Stmt.ifThenElse B S T, s) (S, s)
+  | if_false (B S T s) (hcond : ¬ B s) :
+    SmallStep (Stmt.ifThenElse B S T, s) (T, s)
+  | whileDo (B S s) :
+    SmallStep (Stmt.whileDo B S, s)
+      (Stmt.ifThenElse B (S; Stmt.whileDo B S) Stmt.skip, s)
+
+infixr:100 " ⇒ " => SmallStep
+infixr:100 " ⇒* " => RTC SmallStep
+
+#check absurd
+
+theorem SmallStep_deterministic {Ss Ll Rr}
+      (hl : Ss ⇒ Ll) (hr : Ss ⇒ Rr) :
+    Ll = Rr :=
+    by
+      induction hl generalizing Rr with
+      | assign x a s =>
+        cases hr with
+        | assign _ _ _ => rfl
+      | seq_step S S₁ T s s₁ hS₁ ih =>
+        cases hr with
+        | seq_step S S₂ _ _ s₂ hS₂ =>
+          have heq := ih hS₂
+          injection heq with h1 h2
+          rw [h1, h2]
+        | seq_skip => cases hS₁
+      | seq_skip T s =>
+        cases hr with
+        | seq_step _ S _ _ s' hskip => cases hskip
+        | seq_skip => rfl
+      | if_true B S T s hB =>
+        cases hr with
+        | if_true _ _ _ _ hcond => rfl
+        |if_false _ _ _ _ hcond => exact absurd hB hcond
+      | if_false B S T s hB =>
+        cases hr with
+        | if_true _ _ _ _  hcond => exact absurd hcond hB
+        | if_false _ _ _ _ hcond => rfl
+      | whileDo B S s =>
+        cases hr with
+        | whileDo => rfl
+
 end LoVe
